Defs.v
@@ -7,12 +7,33 @@ Local Open Scope lazy_bool_scope.
 Local Open Scope string_scope.
 Local Open Scope eqb_scope.
 
+(** Names *)
+
+(** Names are coded as string. They will be used both for
+    variables and function symbols and predicate symbols.
+
+    During proofs, these strings may be arbitrary. In case of
+    formula parsing, we'll use the usual syntactic conventions
+    for identifiers : a letter first, then letters or digits or "_".
+    Some symbols will also be accepted as function or predicate
+    symbols, such as "+" "*" "=" "∈". In fact, pretty much
+    anything that doesn't contain the parenthesis characters
+    or the comma. *)
+
+Definition name := string.
+Bind Scope string_scope with name.
+
+(** Variables *)
+
+Definition variable := name.
+Bind Scope string_scope with name.
+
 (** Signatures *)
 
 (** Just in case, a signature that could be infinite *)
 
-Definition function_symbol := string.
-Definition predicate_symbol := string.
+Definition function_symbol := name.
+Definition predicate_symbol := name.
 Definition arity := nat.
 
 Bind Scope string_scope with function_symbol.
@@ -39,11 +60,6 @@ Definition to_infinite sign :=
 
 End Finite.
 
-
-(** In pratice, the symbols could be special characters as "+", or
-    names. In fact, pretty much anything that doesn't contain
-    the parenthesis characters or the comma. *)
-
 Definition peano_sign :=
   {| Finite.funsymbs := [("O",0);("S",1);("+",2);("*",2)];
      Finite.predsymbs := [("=",2)] |}.
@@ -53,60 +69,55 @@ Definition zf_sign :=
      Finite.predsymbs := [("=",2);("∈",2)] |}.
 
 
-(** Variables *)
+(** Sets of names *)
 
-(** Variables are coded as string, and will follow the usual
-    syntactic conventions for identifiers : a letter first, then
-    letters or digits or "_". *)
+Module Names.
+ Include MSetRBT.Make (StringOT).
 
-Definition variable := string.
+ Definition of_list : list name -> t :=
+   fold_right add empty.
 
-Bind Scope string_scope with variable.
+ Fixpoint unions (l: list t) :=
+   match l with
+   | [] => empty
+   | vs::l => union vs (unions l)
+   end.
 
-Module Vars := MSetRBT.Make (StringOT).
+ Definition unionmap {A} (f: A -> t) :=
+   fix unionmap (l:list A) :=
+     match l with
+     | [] => empty
+     | a::l => union (f a) (unionmap l)
+     end.
+
+ Definition map (f:name->name) (s : t) :=
+   fold (fun v => add (f v)) s empty.
+
+ Definition flatmap (f:name->t) (s : t) :=
+   fold (fun v => union (f v)) s empty.
+
+End Names.
 
 (* Prevent incomplete reductions *)
-Arguments Vars.singleton !_.
-Arguments Vars.add !_ !_.
-Arguments Vars.remove !_ !_.
-Arguments Vars.union !_ !_.
-Arguments Vars.inter !_ !_.
-Arguments Vars.diff !_ !_.
+Arguments Names.singleton !_.
+Arguments Names.add !_ !_.
+Arguments Names.remove !_ !_.
+Arguments Names.union !_ !_.
+Arguments Names.inter !_ !_.
+Arguments Names.diff !_ !_.
 
-Definition vars_of_list : list variable -> Vars.t :=
- fold_right Vars.add Vars.empty.
+(** [fresh names] : gives a new name not in the set [names]. *)
 
-Fixpoint vars_unions (l: list Vars.t) :=
- match l with
- | [] => Vars.empty
- | vs::l => Vars.union vs (vars_unions l)
- end.
-
-Definition vars_unionmap {A} (f: A -> Vars.t) :=
- fix flatmap (l:list A) :=
- match l with
- | [] => Vars.empty
- | a::l => Vars.union (f a) (flatmap l)
- end.
-
-Definition vars_map (f:string->string) (vs : Vars.t) :=
-  Vars.fold (fun v => Vars.add (f v)) vs Vars.empty.
-
-Definition vars_flatmap (f:string->Vars.t) (vs : Vars.t) :=
-  Vars.fold (fun v => Vars.union (f v)) vs Vars.empty.
-
-(** [fresh_var vars] : gives a new variable not in the set [vars]. *)
-
-Fixpoint fresh_var_loop (vars:Vars.t) (id:string) n : variable :=
+Fixpoint fresh_loop (names:Names.t) (id:string) n : variable :=
   match n with
   | O => id
-  | S n => if negb (Vars.mem id vars) then id
-           else fresh_var_loop vars (id++"x") n
+  | S n => if negb (Names.mem id names) then id
+           else fresh_loop names (id++"x") n
   end.
 
-Definition fresh_var vars := fresh_var_loop vars "x" (Vars.cardinal vars).
+Definition fresh names := fresh_loop names "x" (Names.cardinal names).
 
-(* Compute fresh_var (Vars.add "x" (Vars.add "y" (Vars.singleton "xx"))). *)
+(* Compute fresh (Names.add "x" (Names.add "y" (Names.singleton "xx"))). *)
 
 
 (** Misc types : operators, quantificators *)
