Countable.v
@@ -1,5 +1,5 @@
-Require Import Ascii Defs Mix Proofs Meta Omega Setoid Morphisms
- NArith.
+Require Import Ascii NArith Omega Setoid Morphisms.
+Require Import Defs Mix NameProofs Meta.
 Import ListNotations.
 Local Open Scope bool_scope.
 Local Open Scope lazy_bool_scope.
