NameProofs.v
@@ -1,0 +1,377 @@
+
+Require Import Ascii Omega MSetFacts MSetProperties
+ Setoid Utils StringUtils Defs.
+Local Open Scope bool_scope.
+Local Open Scope lazy_bool_scope.
+Local Open Scope string_scope.
+Local Open Scope eqb_scope.
+
+Module NamesP := Properties(Names).
+Module NamesF := NamesP.FM.
+Ltac namedec := NamesP.Dec.fsetdec.
+Ltac nameiff := NamesF.set_iff.
+
+Hint Extern 10 => namedec : set.
+
+Lemma InA_In {A} x (l:list A) : InA eq x l <-> In x l.
+Proof.
+ split.
+ rewrite InA_alt. now intros (y & <- & H).
+ apply In_InA; auto with *.
+Qed.
+
+Import Names.
+Import Logic. (* for [eq] *)
+
+Lemma mem_false x vs :
+ ~In x vs -> mem x vs = false.
+Proof.
+ rewrite <- mem_spec. now case mem.
+Qed.
+
+Lemma names_of_list_in l x : In x (of_list l) <-> List.In x l.
+Proof.
+ induction l as [|y l IH]; simpl. namedec.
+ nameiff. intuition.
+Qed.
+
+Lemma unions_in (l: list t) v :
+ In v (unions l) <-> exists vs, In v vs /\ List.In vs l.
+Proof.
+ induction l; simpl.
+ - split. namedec. intros (vs & _ & [ ]).
+ - nameiff. rewrite IHl. split.
+   + intros [H | (vs & H1 & H2)].
+     * exists a; intuition.
+     * exists vs; intuition.
+   + intros (vs & H1 & [->|H2]).
+     * now left.
+     * right; now exists vs.
+Qed.
+
+Lemma unionmap_alt {A} (f: A -> t) (l: list A) :
+ Equal (unionmap f l) (unions (List.map f l)).
+Proof.
+ induction l; simpl.
+ - namedec.
+ - rewrite IHl. namedec.
+Qed.
+
+Lemma unionmap_in {A} (f: A -> t) (l: list A) v :
+ In v (unionmap f l) <-> exists a, In v (f a) /\ List.In a l.
+Proof.
+ rewrite unionmap_alt.
+ rewrite unions_in.
+ split.
+ - intros (vs & H1 & H2).
+   rewrite in_map_iff in H2. destruct H2 as (a & <- & H3).
+   now exists a.
+ - intros (a & H1 & H2). exists (f a); split; auto using in_map.
+Qed.
+
+Lemma unionmap_in' {A} (f: A -> t) (l: list A) a v :
+ In v (f a) -> List.In a l -> In v (unionmap f l).
+Proof.
+ intros. apply unionmap_in. now exists a.
+Qed.
+
+Hint Resolve unionmap_in' : set.
+
+Lemma map_in_aux (f : name -> name) l y acc :
+ In y
+  (List.fold_left (fun vs a => add (f a) vs) l acc) <->
+ (In y acc \/ exists x, f x = y /\ List.In x l).
+Proof.
+ revert acc.
+ induction l as [|a l IH]; intros acc.
+ - simpl. firstorder.
+ - simpl. rewrite IH; clear IH. nameiff.
+   firstorder congruence.
+Qed.
+
+Lemma map_in (f : name -> name) vs y :
+  In y (map f vs) <-> (exists x, f x = y /\ In x vs).
+Proof.
+ unfold map.
+ rewrite fold_spec.
+ rewrite map_in_aux.
+ nameiff.
+ setoid_rewrite NamesF.elements_iff.
+ setoid_rewrite InA_In. intuition.
+Qed.
+
+Lemma map_card_aux (f : name -> name) l acc :
+ (forall x y, List.In x l ->
+              List.In y l -> f x = f y -> x = y) ->
+ (forall x, List.In x l -> ~In (f x) acc) ->
+ NoDupA eq l ->
+ cardinal (List.fold_left (fun vs a => add (f a) vs) l acc) =
+ cardinal acc + List.length l.
+Proof.
+ revert acc.
+ induction l as [|a l IH]; simpl; auto.
+ intros acc Hf Hf' ND.
+ inversion_clear ND.
+ rewrite InA_In in H.
+ rewrite IH; clear IH; auto.
+ rewrite NamesP.add_cardinal_2. omega.
+ apply Hf'; auto.
+ intros x Hx. nameiff. intros [Eq|IN].
+ apply Hf in Eq; auto. congruence.
+ apply Hf' in IN; auto.
+Qed.
+
+Lemma map_cardinal (f : name -> name) vs :
+ (forall x y, In x vs -> In y vs -> f x = f y -> x = y) ->
+ cardinal (map f vs) = cardinal vs.
+Proof.
+ intros Hf.
+ unfold map. rewrite fold_spec.
+ rewrite map_card_aux.
+ - simpl. now rewrite cardinal_spec.
+ - intros x y Hx Hy. apply Hf.
+   now rewrite NamesF.elements_iff, InA_In.
+   now rewrite NamesF.elements_iff, InA_In.
+ - intros x. nameiff. intuition.
+ - apply elements_spec2w.
+Qed.
+
+Lemma unionmap_app {A} f (l l':list A) :
+ Equal (unionmap f (l++l')) (union (unionmap f l) (unionmap f l')).
+Proof.
+ induction l; simpl; namedec.
+Qed.
+
+Lemma unionmap_rev {A} f (l:list A) :
+ Equal (unionmap f (rev l)) (unionmap f l).
+Proof.
+ induction l; simpl. namedec. rewrite unionmap_app.
+ simpl. namedec.
+Qed.
+
+Lemma flatmap_alt (f:name->t) vs :
+ Equal (flatmap f vs) (unionmap f (elements vs)).
+Proof.
+ unfold flatmap.
+ rewrite NamesP.fold_spec_right, <- unionmap_rev.
+ change name with elt.
+ induction (rev (elements vs)); simpl; auto; namedec.
+Qed.
+
+Lemma flatmap_in (f:name->t) vs v :
+  In v (flatmap f vs) <->
+  exists w, In v (f w) /\ In w vs.
+Proof.
+ rewrite flatmap_alt, unionmap_in.
+ setoid_rewrite <- (elements_spec1 vs).
+ now setoid_rewrite InA_In.
+Qed.
+
+Instance flatmap_subset :
+ Proper (eq ==> Subset ==> Subset) flatmap.
+Proof.
+ intros f f' <- s s' E v.
+ rewrite !flatmap_in.
+ intros (w & Hw & Hw'). exists w; auto.
+Qed.
+
+Instance map_proper :
+ Proper (eq ==> Equal ==> Equal) map.
+Proof.
+ unfold map.
+ intros f f' <- s s' E.
+ apply NamesP.fold_equal; auto.
+ - split; eauto with set.
+ - now intros x x' <- y y' <-.
+ - intros x y z. namedec.
+Qed.
+
+Instance flatmap_proper :
+ Proper (eq ==> Equal ==> Equal) flatmap.
+Proof.
+ unfold flatmap.
+ intros f f' <- s s' E.
+ apply NamesP.fold_equal; auto.
+ - split; eauto with set.
+ - now intros x x' <- y y' <-.
+ - intros x y z. namedec.
+Qed.
+
+Lemma flatmap_union (f:name->t) vs vs' :
+ Equal (flatmap f (union vs vs'))
+       (union (flatmap f vs) (flatmap f vs')).
+Proof.
+ intros x. nameiff. rewrite !flatmap_in.
+ setoid_rewrite union_spec. firstorder.
+Qed.
+
+Lemma string_app_empty_r s : s ++ "" = s.
+Proof.
+ induction s. auto. simpl. now f_equal.
+Qed.
+
+Fixpoint prefixes s :=
+  match s with
+  | "" => singleton ""
+  | String a s => add "" (map (String a) (prefixes s))
+  end.
+
+Lemma prefixes_in s u : In u (prefixes s) <-> Prefix u s.
+Proof.
+ revert u.
+ induction s as [|a s IH]; simpl; intros u.
+ - nameiff. split. now intros <-. now inversion 1.
+ - nameiff. rewrite map_in.
+   setoid_rewrite IH.
+   split.
+   + intros [<- | (x & <- & H)]; auto.
+   + inversion_clear 1. now left. right. now eexists.
+Qed.
+
+Definition strict_prefixes s :=
+ remove "" (remove s (prefixes s)).
+
+Lemma prefixes_cardinal s :
+ cardinal (prefixes s) = S (String.length s).
+Proof.
+ induction s as [|a s IH]; simpl.
+ - apply NamesP.singleton_cardinal.
+ - rewrite NamesP.add_cardinal_2.
+   + f_equal. rewrite <- IH.
+     apply map_cardinal.
+     now intros x y _ _ [= ].
+   + rewrite map_in. intros (x & [= ] & _).
+Qed.
+
+Lemma strict_prefixes_cardinal s :
+  cardinal (strict_prefixes s) = pred (String.length s).
+Proof.
+ destruct (string_dec s "").
+ - subst. simpl. unfold strict_prefixes. simpl.
+   apply NamesP.cardinal_Empty. namedec.
+ - unfold strict_prefixes.
+   assert (E := prefixes_cardinal s).
+   rewrite <- (NamesP.remove_cardinal_1 (x:=s)) in E.
+   injection E as E.
+   rewrite <- (NamesP.remove_cardinal_1 (x:="")) in E.
+   now rewrite <- E.
+   + nameiff; split; auto. apply prefixes_in. auto.
+   + apply prefixes_in. apply Prefix_refl.
+Qed.
+
+Lemma subset_equal u v:
+  Subset u v -> cardinal u = cardinal v ->
+  Equal u v.
+Proof.
+ intros SU CA.
+ apply NamesP.subset_antisym; auto.
+ intros x IN.
+ destruct (NamesP.In_dec x u) as [H|H]; auto.
+ generalize (NamesP.subset_cardinal_lt SU IN H). omega.
+Qed.
+
+Lemma string_app_length s s' :
+ String.length (s++s') = String.length s + String.length s'.
+Proof.
+ induction s; simpl; auto.
+Qed.
+
+Lemma prefixes_app s s' :
+  Equal (prefixes (s++s'))
+        (union (prefixes s) (map (append s) (prefixes s'))).
+Proof.
+ intro x.
+ nameiff.
+ rewrite map_in.
+ repeat setoid_rewrite prefixes_in.
+ apply Prefix_app_r.
+Qed.
+
+Lemma prefixes_more s a :
+  Equal (prefixes (s++String a ""))
+        (add (s++String a "") (prefixes s)).
+Proof.
+ rewrite prefixes_app.
+ rewrite NamesP.add_union_singleton.
+ rewrite NamesP.union_sym.
+ intro x.
+ nameiff.
+ rewrite map_in.
+ setoid_rewrite prefixes_in.
+ split; [intros [(y & <- & H)|H] | intros [<-|H]]; auto.
+ - inversion_clear H.
+   + right. rewrite string_app_empty_r. apply Prefix_refl.
+   + inversion_clear H0; auto.
+ - left. exists (String a ""); auto.
+Qed.
+
+Lemma strict_prefixes_more s a :
+  Equal (strict_prefixes (s++String a ""))
+        (remove "" (add s (strict_prefixes s))).
+Proof.
+ unfold strict_prefixes.
+ rewrite prefixes_more.
+ intros x.
+ nameiff. rewrite prefixes_in. intuition; subst.
+ - destruct (string_dec s x); auto.
+ - right. apply Prefix_refl.
+ - assert (String.length (x++String a "") = String.length x).
+   { now f_equal. }
+   rewrite string_app_length in *. simpl in *. omega.
+ - apply Prefix_length in H.
+   rewrite string_app_length in *. simpl in *. omega.
+Qed.
+
+Lemma fresh_loop_ok names id n :
+ (cardinal names < n + String.length id)%nat ->
+ Subset (strict_prefixes id) names ->
+ ~In (fresh_loop names id n) names.
+Proof.
+ revert names id.
+ induction n.
+ - simpl. intros vars id LT SU.
+   assert (E : cardinal (strict_prefixes id) = cardinal vars).
+   { apply NamesP.subset_cardinal in SU.
+     rewrite strict_prefixes_cardinal in *.
+     omega. }
+   apply subset_equal in E; auto. clear SU.
+   rewrite <- E.
+   unfold strict_prefixes. nameiff. intuition.
+ - simpl. intros vars id LT SU.
+   destruct (mem id vars) eqn:ME; simpl.
+   + rewrite mem_spec in ME.
+     apply IHn.
+     * rewrite string_app_length. simpl. omega.
+     * rewrite strict_prefixes_more; auto.
+       { intros x. red in SU. nameiff. intuition. }
+   + rewrite <- mem_spec. now destruct mem.
+Qed.
+
+Lemma fresh_ok names :
+  ~In (fresh names) names.
+Proof.
+ unfold fresh. apply fresh_loop_ok.
+ simpl. omega.
+ change "x" with (""++String "x" "").
+ rewrite strict_prefixes_more.
+ unfold strict_prefixes. simpl. namedec.
+Qed.
+
+Lemma exist_fresh names : exists z, ~In z names.
+Proof.
+ exists (fresh names). apply fresh_ok.
+Qed.
+
+Instance : Proper (Equal ==> eq ==> eq ==> eq) fresh_loop.
+Proof.
+ intros vs vs' EQ id id' <- n n' <-.
+ revert vs vs' EQ id.
+ induction n; cbn; intros vs vs' EQ id; auto.
+ rewrite <- EQ. destruct mem; cbn; auto.
+Qed.
+
+Instance : Proper (Equal ==> eq) fresh.
+Proof.
+ intros vs vs' EQ.
+ unfold fresh. now rewrite <-EQ.
+Qed.
